Clap/Compiler/Vectors.lean
@@ -25,11 +25,44 @@ namespace Clap.Compiler
 --   Sym.Simp.liftTermElabM Term.synthesizeSyntheticMVarsNoPostponing
 --   pure (Expr.app vectorSansProof proof) >>= instantiateMVars
 
-def getElemVectorOfIdx (coll sz : Expr) (idx : ℕ) : Sym.Simp.SimpM Expr := do
+def _root_.Lean.Meta.Sym.getLevelInType (e : Expr) : Sym.SymM Level := do
+  let .succ u ← Sym.getLevel e | throwError m!"getLevelInType - Prop unsupported. Request:\n{e}"
+  return u
+#check Vector.instGetElemNatLt
+def getElemVectorOfIdx (coll t sz : Expr) (idx : ℕ) : Sym.Simp.SimpM Expr := do
   let idx := mkNatLit idx
-  let getElemSansProof ← Sym.shareCommonInc (←Meta.mkAppM ``GetElem.getElem #[coll, idx])
-  let proof := mkApp2 (.const ``Nat.lt []) idx sz
-  Sym.shareCommonInc <| mkAppN getElemSansProof #[←mkSorry proof false]
+  -- instGetElemNatLt
+  -- let getElemSansProof ←
+  --   Sym.shareCommonInc (
+  --     ←Meta.mkAppM ``GetElem.getElem #[coll, idx]
+  --   )
+
+  let collT ← Sym.inferType coll
+
+  let u ← Sym.getLevelInType collT
+  let v ← Sym.getLevelInType q(ℕ)
+  let w ← Sym.getLevelInType t
+
+  -- `λ _x i ↦ i < sz`
+  let valid :=
+    Expr.lam `_x collT
+      (Expr.lam `_i q(ℕ)
+        (mkApp2 (.const ``Nat.lt []) (.bvar 0) sz) .default) .default
+
+  -- `GetElem` instance
+  let inst :=
+    mkApp2 (.const ``Vector.instGetElemNatLt [w]) t sz
+
+  -- `coll[idx]'?proofIsValid`
+  let getElemSansProof ←
+    Sym.shareCommonInc <|
+      mkAppN
+        (.const ``GetElem.getElem [u, v, w])
+        #[collT, q(ℕ), t, valid, inst, coll, idx]
+    
+  let proofIsValid := mkApp2 (.const ``Nat.lt []) idx sz
+
+  Sym.shareCommonInc <| mkAppN getElemSansProof #[←mkSorry proofIsValid false]
 
 def inferVectorProof (vectorSansProof : Expr) : Sym.Simp.SimpM Expr := do
   let .forallE _ argT _ _ ← Sym.inferType vectorSansProof | unreachable!
@@ -49,11 +82,10 @@ def inferVectorProof (vectorSansProof : Expr) : Sym.Simp.SimpM Expr := do
 /--
 TODO: Bad API, no time. (can infer length)
 -/
-def mkVecLit (l : Expr) (len : Expr) : Sym.Simp.SimpM Expr := do
+def mkVecLit (t l len : Expr) : Sym.Simp.SimpM Expr := do
   -- `List.toArray` is not fully-reduced, confuses `Sym` without `unfoldReducible`
-  let array ← mkAppM ``Array.mk #[l]
-  let t := (←inferType array).getAppArgs[0]!
-  let u ← getDecLevel t
+  let u ← Sym.getLevelInType t
+  let array := mkAppN (.const ``Array.mk [u]) #[t, l]
   let vectorSansProof := mkAppN (.const ``_root_.Vector.mk [u]) #[t, len, array]
   let vector ← inferVectorProof vectorSansProof
   Sym.shareCommonInc vector -- TODO: Check if `...inc` is enough.
@@ -71,6 +103,20 @@ def mkVecLit (l : Expr) (len : Expr) : Sym.Simp.SimpM Expr := do
 --     m!"\n{name}[length = {len}][elemType = {t}]\n==>\n{e'}"
 --   Sym.shareCommonInc e'
 
+private def mkListLitAux (nil : Expr) (cons : Expr) : List Expr → Expr
+  | []    => nil
+  | x::xs => mkApp (mkApp cons x) (mkListLitAux nil cons xs)
+
+open Lean Meta Sym in
+def _root_.Lean.Meta.Sym.mkListLit (type : Expr) (xs : List Expr) : SymM Expr := do
+  let u ← Sym.getLevelInType type
+  let nil := mkApp (mkConst ``List.nil [u]) type
+  match xs with
+  | [] => return nil
+  | _  =>
+    let cons := mkApp (mkConst ``List.cons [u]) type
+    return mkListLitAux nil cons xs
+
 def sequenceAsVecExpr (name : Expr) (t sz : Expr) : Sym.Simp.SimpM Expr := do
   let lenSimped := (←Sym.simpWithGround sz).getResultExpr sz
   match lenSimped.nat? with
@@ -82,11 +128,11 @@ def sequenceAsVecExpr (name : Expr) (t sz : Expr) : Sym.Simp.SimpM Expr := do
     trace[Clap.Compile.simp.proc.sequenceAsVecExpr]
       m!"Info: Constructing `Vector _ ({sz})` of ground length {lenSimped}. Request:\n{name}"
   let elems ← Sym.shareCommonInc (
-                ←mkListLit t (←List.range lenSimpedNat |>.mapM (getElemVectorOfIdx name sz))
+                ←mkListLit t (←List.range lenSimpedNat |>.mapM (getElemVectorOfIdx name t sz))
               )
-  let e' ← mkVecLit elems sz
+  let e' ← mkVecLit t elems sz
   trace[Clap.Compile.simp.proc.sequenceAsVecExpr]
-    m!"[vec = \n{name}][length = {sz}][elemType = {t}]\n==>\n{e'}"
+    m!"[vec = {name}][length = {sz}][elemType = {t}]\n==>\n{e'}"
   return e'
 
 -- def needsExploding (e : Expr) : SimpM Bool := do
@@ -167,36 +213,36 @@ lemma abc' : ∀ {α} {vec : Vector α 2}, vec = #v[vec[0], vec[1]] :=
         )
         h
 
--- /--
--- Use with `↓`.
--- -/
--- def dontExplodeVector : Sym.Simp.Simproc := fun e ↦ do
---   let_expr GetElem.getElem _ _ _ _ _ coll _ _ := e | return .rfl
---   unless coll.isFVar && (←inferType coll).isAppOf ``Vector do return .rfl
---   trace[Clap.Compile.simp.kaboom] m!"Done:\n{e}"
---   return .rfl (done := true)
+/--
+Use with `↓`.
+-/
+def dontExplodeVector : Sym.Simp.Simproc := fun e ↦ do
+  let_expr GetElem.getElem _ _ _ _ _ coll _ _ := e | return .rfl
+  unless coll.isFVar && (←inferType coll).isAppOf ``Vector do return .rfl
+  -- trace[Clap.Compile.simp.kaboom] m!"Marked done:\n{e}"
+  return .rfl (done := true)
 
--- /--
--- Use with ↑.
+/--
+Use with ↑.
 
--- TODO: The proof is not `rfl`. One can prove all of these `by aesop (add cases [Vector, Array, List])`,
---       but I'd rather not lift to `aesop` and build the proof by hand (viz. `abc'` above).
--- -/
--- def explodeVector : Sym.Simp.Simproc := fun e ↦ do
---   let t ← inferType e
---   let_expr Vector t sz := t | return .rfl
---   unless e.isFVar do return .rfl
---   let sz' ← Sym.simp sz
---   match (sz'.getResultExpr sz).nat? with
---   | .none => throwError m!"{sz} does not simplify to ground.\nExpr:\n{e}"
---   | .some n => let explodedVec ← (sequenceAsVecExpr e t n).run'
---                trace[Clap.Compile.simp.kaboom] m!"Exploding:\n{e}\n==>\n{explodedVec}"
---                return .step explodedVec (←mkSorry (←mkEq e explodedVec) false)
+TODO: The proof is not `rfl`. One can prove all of these `by aesop (add cases [Vector, Array, List])`,
+      but I'd rather not lift to `aesop` and build the proof by hand (viz. `abc'` above).
+-/
+def explodeVector : Sym.Simp.Simproc := fun e ↦ do
+  let t ← Sym.inferType e
+  let_expr Vector t sz := t | return .rfl
+  unless e.isFVar do return .rfl
+  let sz' ← Sym.simpWithGround sz
+  match (sz'.getResultExpr sz).nat? with
+  | .none => throwError m!"{sz} does not simplify to ground.\nExpr:\n{e}"
+  | .some n => let explodedVec ← (sequenceAsVecExpr e t (sz'.getResultExpr sz)).run'
+               trace[Clap.Compile.simp.kaboom] m!"Exploding:\n{e}\n==>\n{explodedVec}"
+               return .step explodedVec (←mkSorry (←mkEq e explodedVec) false)
 
-def toVectorSequence? (e : Expr) : Sym.Simp.SimpM (Option Expr) := do
+def toVectorSequence? (e : Expr) : Sym.Simp.SimpM (Option (Expr × Expr × Expr)) := do
   unless e.isFVar do return .none
   let_expr Vector t sz := ←Sym.inferType e | return .none
-  return .some (←sequenceAsVecExpr e t sz)
+  return .some ⟨←sequenceAsVecExpr e t sz, t, sz⟩
 
 /-
 Ideally, we'd just use `explodeVector` and `dontExplodeVector`
@@ -210,116 +256,134 @@ of the operations.
 TODO: Generalise.
 -/
 
-open Compiler.Simp
+-- open Compiler.Simp
+-- #check Vector.instHAppendHAddNat
+-- /--
+-- TODO: Proof. Viz. `abc'`.
+-- -/
+-- def explodeVectorAppend : Sym.Simp.Simproc := fun e ↦ do
+--   let_expr HAppend.hAppend α β γ _ a b := e | return .rfl
 
-/--
-TODO: Proof. Viz. `abc'`.
--/
-def explodeVectorAppend : Sym.Simp.Simproc := fun e ↦ do
-  let_expr HAppend.hAppend _ _ _ _ a b := e | return .rfl
+--   let a? ← toVectorSequence? a
+--   let b? ← toVectorSequence? b
+  
+--   if a?.isNone && b?.isNone then return .rfl
 
-  let a? ← toVectorSequence? a
-  let b? ← toVectorSequence? b
-  if a?.isNone && b?.isNone then return .rfl
+--   let_expr Vector ta sza := ←Sym.inferType a | unreachable!
+--   let_expr Vector _tb szb := ←Sym.inferType b | unreachable!
+--   -- `ta` better equal `_tb`
 
-  let append ← reducedAndSharedInc (← mkAppM ``HAppend.hAppend #[a?.getD a, b?.getD b])
-  trace[Clap.Compile.simp.kaboom]
-    m!"\n{e}\n==>\n{append}"
-  return .step append (←mkSorry (←mkEq e append) false)
+--   let a := a?.map Prod.fst |>.getD a
+--   let b := b?.map Prod.fst |>.getD b
 
-/--
-TODO: Proof. Viz. `abc'`.
--/
-def explodeVectorMap : Sym.Simp.Simproc := fun e ↦ do
-  let_expr Vector.map _ _ _ f xs := e | return .rfl
-  -- logWarning m!"Exploding:\n{e}"
+--   let u ← Sym.getLevel α
+--   let v ← Sym.getLevel β
+--   let w ← Sym.getLevel γ
 
-  let xs ← toVectorSequence? xs
-  match xs with
-  | .none => return .rfl
-  | .some xs => let map ← reducedAndSharedInc (←mkAppM ``Vector.map #[f, xs])
-                trace[Clap.Compile.simp.kaboom]
-                  m!"\n{e}\n==>\n{map}"
-                return .step map (←mkSorry (←mkEq e map) false)
+--   let inst := mkAppN (.const ``Vector.instHAppendHAddNat [←Sym.getLevel ta]) #[ta, sza, szb]
 
-/--
-TODO: Proof. Viz. `abc'`.
--/
-def explodeVectorMapIdx : Sym.Simp.Simproc := fun e ↦ do
-  let_expr Vector.mapIdx _ _ _ f xs := e | return .rfl
-  let xs ← toVectorSequence? xs
-  match xs with
-  | .none => return .rfl
-  | .some xs => let mapIdx ← Sym.shareCommonInc (←mkAppM ``Vector.mapIdx #[f, xs])
-                trace[Clap.Compile.simp.kaboom]
-                  m!"\n{e}\n==>\n{mapIdx}"
-                return .step mapIdx (←mkSorry (←mkEq e mapIdx) false)
+--   let append ←
+--     Sym.shareCommonInc
+--       (mkAppN (.const ``HAppend.hAppend [u, v, w]) #[α, β, γ, inst, a, b])
 
-/--
-TODO: Proof. Viz. `abc'`.
--/
-def explodeVectorMapM : Sym.Simp.Simproc := fun e ↦ do
-  let_expr Vector.mapM _ _ _ _ _ f xs := e | return .rfl
-  let xs ← toVectorSequence? xs
-  match xs with
-  | .none => return .rfl
-  | .some xs => let map ← Sym.shareCommonInc (←mkAppM ``Vector.mapM #[f, xs])
-                trace[Clap.Compile.simp.kaboom]
-                  m!"\n{e}\n==>\n{map}"
-                return .step map (←mkSorry (←mkEq e map) false)
+--   trace[Clap.Compile.simp.kaboom]
+--     m!"\n{e}\n==>\n{append}"
 
-/--
-TODO: Proof. Viz. `abc'`.
--/
-def explodeVectorZipWith : Sym.Simp.Simproc := fun e ↦ do
-  let_expr Vector.zipWith _ _ _ _ f a b := e | return .rfl
+--   return .step append (←mkSorry (←mkEq e append) false)
 
-  let a? ← toVectorSequence? a
-  let b? ← toVectorSequence? b
-  if a?.isNone && b?.isNone then return .rfl
+-- /--
+-- TODO: Proof. Viz. `abc'`.
+-- -/
+-- def explodeVectorMap : Sym.Simp.Simproc := fun e ↦ do
+--   let_expr Vector.map _ _ _ f xs := e | return .rfl
+--   -- logWarning m!"Exploding:\n{e}"
 
-  let zipWith ← Sym.shareCommonInc (← mkAppM ``Vector.zipWith #[f, a?.getD a, b?.getD b])
-  trace[Clap.Compile.simp.kaboom]
-    m!"\n{e}\n==>\n{zipWith}"
-  return .step zipWith (←mkSorry (←mkEq e zipWith) false)
+--   let xs ← toVectorSequence? xs
+--   match xs with
+--   | .none => return .rfl
+--   | .some xs => let map ← reducedAndSharedInc (←mkAppM ``Vector.map #[f, xs])
+--                 trace[Clap.Compile.simp.kaboom]
+--                   m!"\n{e}\n==>\n{map}"
+--                 return .step map (←mkSorry (←mkEq e map) false)
 
-/--
-TODO: Proof. Viz. `abc'`.
--/
-def explodeVectorDrop : Sym.Simp.Simproc := fun e ↦ do
-  let_expr Vector.drop _ _ xs k := e | return .rfl
-  let xs ← toVectorSequence? xs
-  match xs with
-  | .none => return .rfl
-  | .some xs => let drop ← reducedAndSharedInc (←mkAppM ``Vector.drop #[xs, k])
-                trace[Clap.Compile.simp.kaboom]
-                  m!"\n{e}\n==>\n{drop}"
-                return .step drop (←mkSorry (←mkEq e drop) false)
+-- /--
+-- TODO: Proof. Viz. `abc'`.
+-- -/
+-- def explodeVectorMapIdx : Sym.Simp.Simproc := fun e ↦ do
+--   let_expr Vector.mapIdx _ _ _ f xs := e | return .rfl
+--   let xs ← toVectorSequence? xs
+--   match xs with
+--   | .none => return .rfl
+--   | .some xs => let mapIdx ← Sym.shareCommonInc (←mkAppM ``Vector.mapIdx #[f, xs])
+--                 trace[Clap.Compile.simp.kaboom]
+--                   m!"\n{e}\n==>\n{mapIdx}"
+--                 return .step mapIdx (←mkSorry (←mkEq e mapIdx) false)
 
-/--
-TODO: Proof. Viz. `abc'`.
--/
-def explodeVectorTake : Sym.Simp.Simproc := fun e ↦ do
-  let_expr Vector.take _ _ xs k := e | return .rfl
-  let xs ← toVectorSequence? xs
-  match xs with
-  | .none => return .rfl
-  | .some xs => let take ← reducedAndSharedInc (←mkAppM ``Vector.take #[xs, k])
-                trace[Clap.Compile.simp.kaboom]
-                  m!"\n{e}\n==>\n{take}"
-                return .step take (←mkSorry (←mkEq e take) false)
-/--
-TODO: Proof. Viz. `abc'`.
--/
-def explodeVectorFoldr : Sym.Simp.Simproc := fun e ↦ do
-  let_expr Vector.foldr _ _ _ f init xs := e | return .rfl
-  let xs ← toVectorSequence? xs
-  match xs with
-  | .none => return .rfl
-  | .some xs => let foldr ← Sym.shareCommonInc (←mkAppM ``Vector.foldr #[f, init, xs])
-                trace[Clap.Compile.simp.kaboom]
-                  m!"\n{e}\n==>\n{foldr}"
-                return .step foldr (←mkSorry (←mkEq e foldr) false)
+-- /--
+-- TODO: Proof. Viz. `abc'`.
+-- -/
+-- def explodeVectorMapM : Sym.Simp.Simproc := fun e ↦ do
+--   let_expr Vector.mapM _ _ _ _ _ f xs := e | return .rfl
+--   let xs ← toVectorSequence? xs
+--   match xs with
+--   | .none => return .rfl
+--   | .some xs => let map ← Sym.shareCommonInc (←mkAppM ``Vector.mapM #[f, xs])
+--                 trace[Clap.Compile.simp.kaboom]
+--                   m!"\n{e}\n==>\n{map}"
+--                 return .step map (←mkSorry (←mkEq e map) false)
+
+-- /--
+-- TODO: Proof. Viz. `abc'`.
+-- -/
+-- def explodeVectorZipWith : Sym.Simp.Simproc := fun e ↦ do
+--   let_expr Vector.zipWith _ _ _ _ f a b := e | return .rfl
+
+--   let a? ← toVectorSequence? a
+--   let b? ← toVectorSequence? b
+--   if a?.isNone && b?.isNone then return .rfl
+
+--   let zipWith ← Sym.shareCommonInc (← mkAppM ``Vector.zipWith #[f, a?.getD a, b?.getD b])
+--   trace[Clap.Compile.simp.kaboom]
+--     m!"\n{e}\n==>\n{zipWith}"
+--   return .step zipWith (←mkSorry (←mkEq e zipWith) false)
+
+-- /--
+-- TODO: Proof. Viz. `abc'`.
+-- -/
+-- def explodeVectorDrop : Sym.Simp.Simproc := fun e ↦ do
+--   let_expr Vector.drop _ _ xs k := e | return .rfl
+--   let xs ← toVectorSequence? xs
+--   match xs with
+--   | .none => return .rfl
+--   | .some xs => let drop ← reducedAndSharedInc (←mkAppM ``Vector.drop #[xs, k])
+--                 trace[Clap.Compile.simp.kaboom]
+--                   m!"\n{e}\n==>\n{drop}"
+--                 return .step drop (←mkSorry (←mkEq e drop) false)
+
+-- /--
+-- TODO: Proof. Viz. `abc'`.
+-- -/
+-- def explodeVectorTake : Sym.Simp.Simproc := fun e ↦ do
+--   let_expr Vector.take _ _ xs k := e | return .rfl
+--   let xs ← toVectorSequence? xs
+--   match xs with
+--   | .none => return .rfl
+--   | .some xs => let take ← reducedAndSharedInc (←mkAppM ``Vector.take #[xs, k])
+--                 trace[Clap.Compile.simp.kaboom]
+--                   m!"\n{e}\n==>\n{take}"
+--                 return .step take (←mkSorry (←mkEq e take) false)
+-- /--
+-- TODO: Proof. Viz. `abc'`.
+-- -/
+-- def explodeVectorFoldr : Sym.Simp.Simproc := fun e ↦ do
+--   let_expr Vector.foldr _ _ _ f init xs := e | return .rfl
+--   let xs ← toVectorSequence? xs
+--   match xs with
+--   | .none => return .rfl
+--   | .some xs => let foldr ← Sym.shareCommonInc (←mkAppM ``Vector.foldr #[f, init, xs])
+--                 trace[Clap.Compile.simp.kaboom]
+--                   m!"\n{e}\n==>\n{foldr}"
+--                 return .step foldr (←mkSorry (←mkEq e foldr) false)
 
 -- /--
 -- TODO: Thought experiment to explode on demand.
