Clap/Compiler/Wheels.lean
@@ -67,7 +67,11 @@ initialize Lean.registerTraceClass `Clap.Compile.simp.proc.evalGround (inherited
 
 initialize Lean.registerTraceClass `Clap.Compile.simp.proc.vector_getElem_mk (inherited := true)
 
-initialize Lean.registerTraceClass `Clap.Compile.simp.proc.vector_mapM_mk_cons (inherited := true)
+initialize Lean.registerTraceClass `Clap.Compile.simp.proc.vector_mk_zipWith_mk (inherited := true)
+
+initialize Lean.registerTraceClass `Clap.Compile.simp.proc.vector_mapM_mk (inherited := true)
+
+initialize Lean.registerTraceClass `Clap.Compile.simp.proc.preprocess (inherited := true)
 
 initialize Lean.registerTraceClass `Clap.Compile.simp.proc.seemsTotallySafeInDTT (inherited := true)
 
